sketch proof for `L_D'' not in DTIME(t)`, adapt definition
requires assumption that `t` is superlinear (`lemma L0_t` already requires that `t` is at least cubic)

papers/116_stefan_rass/LD_Issues.thy
@@ -3,6 +3,10 @@ theory LD_Issues
 begin
 
 
+section\<open>Alternative \<open>L\<^sub>D\<close> (Bridge to Lemma 4.6)\<close>
+
+subsection\<open>Encoding\<close>
+
 \<comment> \<open>Decode a pair of \<open>(l, x) \<in> \<nat> \<times> {0,1}*\<close> from its encoded form \<open>w \<in> {0,1}*\<close>.
 
   The encoding defined by this should have \<open>l\<close> encoded in the upper (more significant) bits of \<open>l\<parallel>x\<close>.
@@ -30,6 +34,42 @@ abbreviation decode_pair :: "word \<Rightarrow> nat \<times> word"
   where "decode_pair w \<equiv> (decode_pair_l w, decode_pair_x w)"
 
 
+definition rev_suffix_len :: "word \<Rightarrow> nat"
+  where "rev_suffix_len w = length w + 9"
+
+definition encode_pair :: "nat \<Rightarrow> word \<Rightarrow> word"
+  where "encode_pair l x = (let w' = x @ [False] @ True \<up> l in
+            False \<up> (rev_suffix_len w') @ w')"
+
+
+lemma encode_pair_altdef:
+  "encode_pair l x = False \<up> (length x + l + 10) @ x @ [False] @ True \<up> l"
+  unfolding encode_pair_def rev_suffix_len_def Let_def by simp
+
+lemma strip_sq_pad_pair:
+  fixes l x
+  defines w: "w \<equiv> encode_pair l x"
+    and w': "w' \<equiv> x @ [False] @ True \<up> l"
+  shows "strip_sq_pad w = w'"
+proof -
+  let ?lw = "length w" and ?lw' = "length w'"
+  have lw: "?lw = 2 * ?lw' + 9" unfolding w w' encode_pair_altdef by simp
+  have lwh: "5 + ?lw div 2 = rev_suffix_len w'" unfolding lw rev_suffix_len_def by simp
+  show "strip_sq_pad w = w'" unfolding strip_sq_pad_def suffix_len_def lwh
+    unfolding w encode_pair_def Let_def w'[symmetric] by simp
+qed
+
+lemma decode_encode_pair:
+  fixes l x
+  defines w: "w \<equiv> encode_pair l x"
+  shows "decode_pair w = (l, x)"
+proof (unfold prod.inject, intro conjI)
+  have rw: "rev (strip_sq_pad w) = True \<up> l @ False # rev x" unfolding w strip_sq_pad_pair by force
+  show "decode_pair_l w = l" unfolding decode_pair_l_def rw by (subst takeWhile_tail) auto
+  show "decode_pair_x w = x" unfolding decode_pair_x_def rw by (subst dropWhile_append3) auto
+qed
+
+
 lemma pair_adj_sq_eq:
   fixes w
   defines w': "w' \<equiv> adj_sq\<^sub>w w"
@@ -50,6 +90,8 @@ proof -
     unfolding decode_pair_x_def decode_pair_l_def sq_pad_eq ..
 qed
 
+
+subsection\<open>Definition\<close>
 
 context tht_assms
 begin
@@ -74,12 +116,12 @@ definition L\<^sub>D'' :: lang
   where "L\<^sub>D'' \<equiv> {w.
       let (l, x) = decode_pair w;
           v = drop (length x - l) x;
-          M\<^sub>v = decode_TM (strip_al_prefix v) in
+          M\<^sub>v = TM_decode_pad v in
       rejects M\<^sub>v v \<and> is_final (steps0 (1, <v>\<^sub>t\<^sub>p) M\<^sub>v (tcomp\<^sub>w T x))
     }"
 
 definition L\<^sub>0'' :: lang
-  where [simp]: "L\<^sub>0'' \<equiv> L\<^sub>D'' \<inter> SQ"
+  where "L\<^sub>0'' \<equiv> L\<^sub>D'' \<inter> SQ"
 
 
 lemma L\<^sub>D''_adj_sq_iff:
@@ -97,17 +139,114 @@ lemma L\<^sub>D''_L\<^sub>0''_adj_sq_iff:
   unfolding L\<^sub>0''_def w' using len[THEN L\<^sub>D''_adj_sq_iff] adj_sq_word_correct by blast
 
 
+subsection\<open>\<open>L\<^sub>D'' \<notin> DTIME(t)\<close> via Reduction to \<open>L\<^sub>D\<close>\<close>
+
+definition reduce_LD_LD'' :: "word \<Rightarrow> word"
+  where "reduce_LD_LD'' w \<equiv> encode_pair (length w) w"
+
+lemma reduce_LD_LD''_len: "length (reduce_LD_LD'' w) = 4 * length w + 11"
+  unfolding reduce_LD_LD''_def encode_pair_def rev_suffix_len_def by auto
+
+lemma reduce_LD_LD''_correct:
+  fixes w
+  defines w'': "w'' \<equiv> reduce_LD_LD'' w"
+  shows "w'' \<in> L\<^sub>D'' \<longleftrightarrow> w \<in> L\<^sub>D"
+proof -
+  let ?M\<^sub>w = "TM_decode_pad w"
+  have "w'' \<in> L\<^sub>D'' \<longleftrightarrow> rejects ?M\<^sub>w w \<and> time_bounded_word T ?M\<^sub>w w"
+    unfolding L\<^sub>D''_def w'' reduce_LD_LD''_def mem_Collect_eq decode_encode_pair
+    unfolding diff_self_eq_0 drop_0 Let_def prod.case unfolding time_bounded_altdef ..
+  also have "... \<longleftrightarrow> w \<in> L\<^sub>D" unfolding LD_def mem_Collect_eq Let_def ..
+  finally show ?thesis .
+qed
+
+
+end \<comment> \<open>context \<^locale>\<open>tht_assms\<close>\<close>
+context tht_sq_assms begin
+
+
+\<comment> \<open>The following proof is similar to that of @{thm tht_sq_assms.L0_t}.\<close>
 lemma L\<^sub>D''_t: "L\<^sub>D'' \<notin> DTIME(t)"
-  sorry (* TODO *)
+proof (rule ccontr, unfold not_not)
+  assume "L\<^sub>D'' \<in> DTIME(t)"
+  then obtain M'' where "decides M'' L\<^sub>D''" and "time_bounded t M''" (* and "tm_wf0 M'" *) ..
+
+  \<comment> \<open>Assume that \<^const>\<open>reduce_LD_LD''\<close> can be realized by a TM in time \<open>O(n)\<close>.\<close>
+  define T\<^sub>R where "T\<^sub>R \<equiv> \<lambda>n::nat. n"
+  obtain M\<^sub>R where "tm_wf0 M\<^sub>R"
+    and M\<^sub>R_correct: "\<And>w. {input w} M\<^sub>R {input (reduce_LD_LD'' w)}"
+    and "time_bounded T\<^sub>R M\<^sub>R"
+    sorry
+
+  define M where "M \<equiv> M\<^sub>R |+| M''"
+  define t' where "t' = (\<lambda>n. tcomp T\<^sub>R n + tcomp t n)"
+
+  have "L\<^sub>D \<in> DTIME(t')"
+  proof (intro in_dtimeI allI)
+    fix w :: word
+
+    from \<open>decides M'' L\<^sub>D''\<close> have "decides_word M'' L\<^sub>D'' (reduce_LD_LD'' w)" ..
+    moreover have "reduce_LD_LD'' w \<in> L\<^sub>D'' \<longleftrightarrow> w \<in> L\<^sub>D" by (rule reduce_LD_LD''_correct)
+    ultimately show "decides_word M L\<^sub>D w" unfolding M_def
+      using M\<^sub>R_correct[of w] \<open>tm_wf0 M\<^sub>R\<close> by (rule reduce_decides)
+
+    \<comment> \<open>This second part (M is \<open>t'\<close>-time-bounded) is considerably harder to show
+      than for @{thm tht_sq_assms.L0_t}.
+      Since the length of \<^term>\<open>reduce_LD_LD'' w\<close> is always greater than the length of \<^term>\<open>w\<close>
+      (@{thm reduce_LD_LD''_len}),
+      the existing @{thm reduce_time_bounded} does not hold in this case.
+
+      Evaluating the time complexity given the differing word-lengths yields a new
+      \<open>t'(n) := T\<^sub>R(n) + t(4n + 11)\<close>.
+      The speed-up theorem does not help here, since for super-polynomial \<open>t\<close>,
+      \<open>t(4n + 11)\<close> is not proportional to \<open>t(n)\<close>.\<close>
+
+    from \<open>time_bounded t M''\<close> have "time_bounded_word t M'' (reduce_LD_LD'' w)" ..
+    moreover from \<open>time_bounded T\<^sub>R M\<^sub>R\<close> have "time_bounded_word T\<^sub>R M\<^sub>R w" ..
+    ultimately show "time_bounded_word t' M w" unfolding M_def t'_def
+      using M\<^sub>R_correct reduce_LD_LD''_len sorry
+  qed
+
+  have t'_t: "real (t' n) \<le> 4 * real (t n)" if "n \<ge> 1" for n
+  proof -
+    have "tcomp T\<^sub>R n = n + 1" unfolding T\<^sub>R_def max_def ceiling_of_nat by simp
+    then have "tcomp T\<^sub>R n + tcomp t n = (n + 1) + tcomp t n" by simp
+    also have "... \<le> 2 * tcomp t n" unfolding mult_2 add_le_cancel_right by simp
+    finally have "t' n \<le> 2 * tcomp t n" unfolding t'_def of_nat_le_iff .
+
+    also have "... \<le> 2 * (2 * t n)"
+    proof (intro mult_le_mono2)
+      have "tcomp t n \<le> tcomp (\<lambda>n. 2 * t n) n"
+        unfolding ceiling_of_nat nat_int by (intro max.mono) auto
+      also have "... = 2 * t n"
+      proof -
+        have "n + 1 \<le> 2 * n" using \<open>n \<ge> 1\<close> by simp
+        also have "... \<le> 2 * t n" using t_min by simp
+        finally have "n + 1 \<le> 2 * t n" .
+        then show ?thesis unfolding ceiling_of_nat nat_int by (fact max_absorb2)
+      qed
+      finally show "tcomp t n \<le> 2 * t n" .
+    qed
+    finally have "t' n \<le> 4 * t n" by simp
+    then have "real (t' n) \<le> real (4 * t n)" by (fact of_nat_mono)
+    also have "... = 4 * real (t n)" by simp
+    finally show ?thesis .
+  qed
+  then have "L\<^sub>D \<in> DTIME(\<lambda>n. 4 * real (t n))" using \<open>L\<^sub>D \<in> DTIME(t')\<close> by (rule DTIME_mono_ae)
+
+  \<comment> \<open>With the current assumptions, \<open>t\<close> is not necessarily super-linear.
+    A similar requirement exists in the proof of @{thm L0_t} (and `L0''_t`, see below),
+    that requires \<open>t\<close> to be at least cubic.\<close>
+  moreover have "\<forall>N. \<exists>n'. \<forall>n\<ge>n'. N \<le> real (t n) / real n" sorry
+  ultimately have "L\<^sub>D \<in> DTIME(t)" by (intro DTIME_speed_up_rev[of 4 t]) auto
+
+  moreover from time_hierarchy have "L\<^sub>D \<notin> DTIME(t)" ..
+  ultimately show False by contradiction
+qed
 
 lemma L\<^sub>D''_T: "L\<^sub>D'' \<in> DTIME(T)"
   sorry (* TODO *)
 
-end \<comment> \<open>context \<^locale>\<open>tht_assms\<close>\<close>
-
-
-context tht_sq_assms
-begin
 
 text\<open>Lemma 4.6. Let \<open>t\<close>, \<open>T\<close> be as in Assumption 4.4 and assume \<open>T(n) \<ge> n\<^sup>3\<close>.
   Then, there exists a language \<open>L\<^sub>0 \<in> DTIME(T) - DTIME(t)\<close> for which \<open>dens\<^sub>L\<^sub>0(x) \<le> \<surd>x\<close>.\<close>
@@ -149,7 +288,13 @@ proof (rule ccontr, unfold not_not)
   then have "L\<^sub>D'' \<in> DTIME(t)" sorry
   \<comment> \<open>This is not correct, since \<^term>\<open>t\<close> could be arbitrarily small.
     Let \<open>t(n) = n\<close> and \<open>T(n) = n\<^sup>3\<close>. Then \<open>DTIME(t)\<close> is limited by \<open>tcomp t n = n + 1\<close>
-    and \<open>DTIME(T)\<close> by \<open>tcomp t n = n\<^sup>3\<close> (for \<open>n > 1\<close>).\<close>
+    and \<open>DTIME(T)\<close> by \<open>tcomp t n = n\<^sup>3\<close> (for \<open>n > 1\<close>).
+
+    For speed-up to help in this case, \<^term>\<open>t\<close> must grow at least as fast as \<^term>\<open>T\<^sub>R\<close>.
+    (also, \<^term>\<open>t\<close> must be super-linear. See @{thm linear_time_speed_up}})
+    \<^term>\<open>T\<^sub>R\<close> is assumed to be \<open>n\<^sup>3\<close>, which allows a naive algorithm for \<^const>\<open>adj_square\<close>.
+    According to Wikipedia, the currently optimal algorithm for computing the square root on a TM
+    seems to be Newton's method with Harvey-Hoeven multiplication with complexity \<open>O(n log(n))\<close>.\<close>
 
   moreover have "L\<^sub>D'' \<notin> DTIME(t)" by (fact L\<^sub>D''_t)
   ultimately show False by contradiction
